src/encode_relation.v
@@ -1,0 +1,64 @@
+From stdpp Require Import countable.
+From iris.base_logic.lib Require Import own.
+
+From self Require Import extra.
+
+Section encode_relation.
+  Context `{Countable A}.
+  Implicit Type (R : relation2 A).
+
+  Definition encode_relation R : relation2 positive :=
+    λ (a b : positive), default False (R <$> decode a <*> decode b).
+
+  Lemma encode_relation_iff R (a b : A) :
+    R a b ↔ (encode_relation R) (encode a) (encode b).
+  Proof.
+    rewrite /encode_relation.
+    rewrite !decode_encode.
+    reflexivity.
+  Qed.
+
+  (* If we know that two encoded values are related by an encoded relation, then
+  we can "recover" related unencoded values taht are related by the unencoded
+  relation. *)
+  Lemma encode_relation_inv R ea eb :
+    (encode_relation R) ea eb →
+    ∃ a b, decode ea = Some a ∧ decode eb = Some b ∧ R a b.
+  Proof.
+    rewrite /encode_relation.
+    destruct (decode ea) as [|], (decode eb) as [|]; try done.
+    intros ?. eexists _, _. done.
+  Qed.
+
+  Lemma encode_relation_decode_iff R ea eb (a b : A) :
+    decode ea = Some a →
+    decode eb = Some b →
+    (encode_relation R) ea eb ↔ R a b.
+  Proof. rewrite /encode_relation. intros -> ->. done. Qed.
+
+  Lemma encode_relation_decode_iff_1 R ea eb (a b : A) :
+    decode ea = Some a →
+    decode eb = Some b →
+    (encode_relation R) ea eb →
+    R a b.
+  Proof. rewrite /encode_relation. intros -> ->. done. Qed.
+
+  Lemma encode_relation_decode_iff_2 R ea eb (a b : A) :
+    decode ea = Some a →
+    decode eb = Some b →
+    R a b →
+    (encode_relation R) ea eb.
+  Proof. rewrite /encode_relation. intros -> ->. done. Qed.
+
+  Global Instance encode_relation_trans R :
+    Transitive R → Transitive (encode_relation R).
+  Proof.
+    intros T. intros encX encY encZ.
+    intros (x & y & decX & decY & Rxy)%encode_relation_inv.
+    intros (? & z & ? & decZ & Ryz)%encode_relation_inv.
+    simplify_eq.
+    eapply encode_relation_decode_iff; [done|done|].
+    etrans; done.
+  Qed.
+
+End encode_relation.
